theories/microgv/definitions.v
@@ -1,0 +1,67 @@
+From diris.microgv Require Export langdef.
+
+(* The definition of the set of barrier references in an expression. *)
+Fixpoint expr_refs e :=
+  match e with
+  | Val v => val_refs v
+  | Var x => ∅
+  | Fun x e => expr_refs e
+  | App e1 e2 => expr_refs e1 ∪ expr_refs e2
+  | Unit => ∅
+  | Pair e1 e2 => expr_refs e1 ∪ expr_refs e2
+  | LetPair e1 e2 => expr_refs e1 ∪ expr_refs e2
+  | Sum i e => expr_refs e
+  | MatchSum n e es => expr_refs e ∪ fin_union n (expr_refs ∘ es)
+  | Fork e => expr_refs e
+  end
+with val_refs v :=
+  match v with
+  | FunV x e => expr_refs e
+  | UnitV => ∅
+  | PairV v1 v2 => val_refs v1 ∪ val_refs v2
+  | SumV i v => val_refs v
+  | BarrierV i => {[ i ]}
+  end.
+
+(* Paper definition 2 *)
+Definition expr_waiting e j := ∃ k v, ctx k ∧ e = k (App (Val $ BarrierV j) (Val v)).
+
+Definition waiting (ρ : cfg) (i j : nat) :=
+  match ρ !! i, ρ !! j with
+  | Some (Thread e), Some Barrier => expr_waiting e j
+  | Some Barrier, Some (Thread e) => i ∈ expr_refs e ∧ ¬ expr_waiting e i
+  | _,_ => False
+  end.
+
+(* These definitions are not explicitly given in the paper, but we factor them out in Coq *)
+Definition can_step (ρ : cfg) (i : nat) := ∃ ρ', step i ρ ρ'.
+Definition inactive (ρ : cfg) (i : nat) := ρ !! i = None.
+
+(* Paper definition 3 *)
+Record deadlock (ρ : cfg) (s : nat -> Prop) := {
+  dl_nostep i : s i -> ¬ can_step ρ i;
+  dl_waiting i j : waiting ρ i j -> s i -> s j;
+}.
+
+(* Paper definition 4 *)
+Definition deadlock_free (ρ : cfg) :=
+  ∀ s, deadlock ρ s -> ∀ i, s i -> inactive ρ i.
+
+(* Paper definition 5 *)
+Inductive reachable (ρ : cfg) : nat -> Prop :=
+  | Can_step_reachable i :
+      can_step ρ i -> reachable ρ i
+  | Waiting_reachable i j :
+      waiting ρ i j -> reachable ρ j -> reachable ρ i.
+
+(* Paper definition 6 *)
+Definition fully_reachable (ρ : cfg) :=
+  ∀ i, inactive ρ i ∨ reachable ρ i.
+
+(* Paper definition 8 *)
+Definition global_progress (ρ : cfg) :=
+  (∀ i, inactive ρ i) ∨ (∃ i, can_step ρ i).
+
+(* Paper definition 9 *)
+Definition type_safety (ρ : cfg) :=
+  ∀ i, inactive ρ i ∨ can_step ρ i ∨ ∃ j, waiting ρ i j.
